Change star compilation

regex/Regex/NFA/Compile/Basic.lean
@@ -10,9 +10,7 @@ public section
 namespace Regex.NFA
 
 def pushNode (nfa : NFA) (node : Node) : NFA :=
-  let start := nfa.size
-  let nodes := nfa.nodes.push node
-  ⟨nodes, start⟩
+  ⟨nfa.nodes.push node⟩
 
 @[simp, grind =]
 theorem pushNode_size {nfa : NFA} {node : Node} :
@@ -23,7 +21,7 @@ theorem pushNode_size {nfa : NFA} {node : Node} :
 theorem pushNode_get_lt {nfa : NFA} {node : Node}
   (i : Nat) (h : i < nfa.size) :
   (nfa.pushNode node)[i]'(Nat.lt_trans h (by simp only [pushNode_size, Nat.lt_add_one])) = nfa[i] := by
-  simp [pushNode, get_eq_nodes_get]
+  simp only [pushNode, get_eq_nodes_get]
   rw [Array.getElem_push_lt]
 
 @[simp, grind =]
@@ -41,7 +39,19 @@ theorem pushNode_get {nfa : NFA} {node : Node}
   | inr eq => simp [eq]
 
 @[simp, grind =]
-theorem pushNode_start_eq {nfa : NFA} {node : Node} : (nfa.pushNode node).start = nfa.size := (rfl)
+theorem pushNode_start {nfa : NFA} {node : Node} :
+  (nfa.pushNode node).start = nfa.size := by
+  grind
+
+@[grind! .]
+theorem pushNode_wf {nfa : NFA} {node : Node} (wf : nfa.WellFormed) (inBounds : node.inBounds (nfa.size + 1)) :
+  (nfa.pushNode node).WellFormed := by
+  refine WellFormed.iff.mpr ⟨by grind, ?_⟩
+  simp only [pushNode_size, pushNode_get]
+  intro i h
+  split
+  next h => exact Node.inBounds_of_inBounds_of_le (wf.inBounds i h) (Nat.le_succ _)
+  next => exact inBounds
 
 /--
   Compile a Regex and append the resulting nodes to the NFA. The nodes will transition to `next` on match.
@@ -52,16 +62,16 @@ def pushRegex (nfa : NFA) (next : Nat) : Expr → NFA
   | .anchor a => nfa.pushNode (.anchor a next)
   | .char c => nfa.pushNode (.char c next)
   | .classes cs => nfa.pushNode (.sparse cs next)
-  | .group index r =>
+  | .group index e =>
     -- push the closing save node first
     let nfa' := nfa.pushNode (.save (2 * index + 1) next)
-    let nfa'' := nfa'.pushRegex nfa'.start r
+    let nfa'' := nfa'.pushRegex nfa'.start e
     nfa''.pushNode (.save (2 * index) nfa''.start)
-  | .alternate r₁ r₂ =>
+  | .alternate e₁ e₂ =>
     -- TODO: it feels better to compile r₂ first to align with concat
-    let nfa₁ := nfa.pushRegex next r₁
+    let nfa₁ := nfa.pushRegex next e₁
     let start₁ := nfa₁.start
-    let nfa₂ := nfa₁.pushRegex next r₂
+    let nfa₂ := nfa₁.pushRegex next e₂
     let start₂ := nfa₂.start
 
     let split := Node.split start₁ start₂
@@ -70,26 +80,21 @@ def pushRegex (nfa : NFA) (next : Nat) : Expr → NFA
   | .concat r₁ r₂ =>
     let nfa₂ := nfa.pushRegex next r₂
     nfa₂.pushRegex nfa₂.start r₁
-  | .star greedy r =>
-    let start := nfa.size
+  | .star greedy e =>
+    let patchAt := nfa.size
     -- We need to generate a placeholder node first. We use `fail` for it because
     -- 1. We want to make sure `done` does not appear except at the first node.
     -- 2. variants without data are represented as a boxed integer so there is one less allocation.
     let placeholder := nfa.pushNode .fail
-    let compiled := placeholder.pushRegex start r
+    let compiled := placeholder.pushRegex patchAt e
+    let split := if greedy then .split compiled.start next else .split next compiled.start
+    let quest := compiled.pushNode split
 
-    let split :=
-      if greedy then
-        .split compiled.start next
-      else
-        .split next compiled.start
     -- While we know that `pushRegex` increase the size and hence this `setIfInBounds` is always
     -- in bounds, we don't use that information to eliminate the bounds check. This is because
     -- it requires changing the return type to `{ nfa' : NFA // nfa.size < nfa'.size }`
     -- which is much more inconvenient to work with.
-    let patched := compiled.nodes.setIfInBounds start split
-
-    ⟨patched, start⟩
+    ⟨quest.nodes.setIfInBounds patchAt split⟩
 
 def compile (r : Expr) : NFA := done.pushRegex 0 r
 
